otbn_model/code/addc512_lemmas.dfy
@@ -8,48 +8,6 @@ module addc512_lemmas {
     import opened powers
     import opened congruences
 
-    lemma single_digit_lemma_0(a: nat, b: nat, u: nat)
-        requires a <= u;
-        requires b <= u;
-        ensures a * b <= u * u;
-    {
-        assert true;
-    }
-
-    lemma single_digit_lemma_1(a: nat, b: nat, c: nat, u: nat)
-        requires a <= u;
-        requires b <= u;
-        requires c <= u;
-        ensures a * b + c < (u + 1) * (u + 1);
-    {
-        calc <= {
-            a * b + c;
-            { single_digit_lemma_0(a, b, u); }
-            u * u + c;
-            u * u + u;
-            u * (u + 1);
-            (u + 1) * (u + 1);
-        }
-    }
-
-    lemma single_digit_lemma_2(a: nat, b: nat, c: nat, d: nat, u: nat)
-        requires a <= u;
-        requires b <= u;
-        requires c <= u;
-        requires d <= u;
-        ensures a * b + c + d < (u + 1) * (u + 1);
-    {
-        calc <= {
-            a * b + c + d;
-            { single_digit_lemma_0(a, b, u); }
-            u * u + c + d;
-            u * u + u + u;
-            u * u + 2 * u;
-            u * u + 2 * u + 1;
-            (u + 1) * (u + 1);
-        }
-    }
-
     lemma addc_256_op_lemma(
         x: uint256, y: uint256, z: uint256, c: uint1)
         requires (z, c) == uint256_addc(x, y, 0);
